Arithmetic/theories/Languages/MiniGMP/Semantics.v
@@ -1,4 +1,5 @@
-From Coq Require Import Strings.String ZArith.ZArith BinaryString.
+From Coq Require Import ZArith.ZArith.
+From Coq.Strings Require Import String BinaryString.
 
 From RAC Require Import Utils Environnement.
 From RAC.Languages Require Import Syntax.
@@ -22,7 +23,7 @@ Section GMPSemantics.
 
     Inductive _gmp_stmt_sem  (fe:rac_prog_fenv) (ev:Env) :  gmp_statement -> Env -> Prop := 
         | S_init x (l:location) u:
-            (forall v, ev v <> Some (Def (VMpz (Some l)))) ->
+            fresh_location ev l ->
             ev x = Some (Undef (UMpz u)) ->
             ev |= <(init(x))> => ev <| env ; vars ::= {{x\Def (VMpz (Some l))}} |> <| mstate ::= {{l\Defined 0}} |>
         
@@ -41,7 +42,7 @@ Section GMPSemantics.
             ev.(mstate) n = Some (Defined z) ->
             ev |= <(set_z(x,y))> => ev <| mstate ::= {{a\Defined z}} |> 
 
-        | S_get_int x y ly zy (ir:Int.inRange zy) :
+        | S_get_int x y ly zy (ir:MI.inRange zy) :
             ev y = Some (Def (VMpz (Some ly))) ->
             ev.(mstate) ly = Some (Defined zy) -> 
             ev |= <(x = get_int(y))> => ev <| env ; vars ::= {{x\VInt (zy ⁱⁿᵗ ir) : 𝕍}} |>
@@ -71,52 +72,13 @@ Section GMPSemantics.
             ev r = Some (Def (VMpz (Some lr))) -> (* not in paper *)
             ev |= fsl_to_gmp_op bop r x y => ev <| mstate ::= {{lr\Defined (⋄ (□ bop) zx zy) }} |>
 
-        | S_Scope decls (s:@c_statement _gmp_statement _gmp_t) ev_s ev_s':
-            (*
-                - A scope has var declarations that gets dropped at the end, except the memory state. 
-                - This was missing in the original paper but required in the translation 
-                as we must create a scope when we translate the assertions 
-                - Note it complicate things because the statement are c instructions, not just gmp ones.
-            *)
-            declare_gmp_vars ev (list_to_ensemble decls) ev_s ->
-            @generic_stmt_sem _gmp_statement _gmp_t _gmp_stmt_sem _gmp_stmt_vars fe ev_s s ev_s' -> 
-            ev |= GMP_Scope decls s =>  ev <| mstate := ev_s' |>
-
 
     where "ev |= s => ev'" := (_gmp_stmt_sem fe (ev:Env) (s:_gmp_statement) (ev':Env)) : ext_gmp_stmt_sem_scope.
 
-    Section Induction.
-
-        (* Variable P : Env -> 𝐒 -> Env -> Prop.
-        Variable P1 : forall x (l:location) u,
-            (forall v, ev v <> Some (Def (VMpz (Some l)))) ->
-            ev x = Some (Undef (UMpz u)) ->
-            (ev |= <(init(x))> => ev <| env ; vars ::= {{x\Def (VMpz (Some l))}} |> <| mstate ::= {{l\Defined 0}} |>) f
-        .
-        
-        Fixpoint _gmpt_stmt_sem_full_ind f ev s ev' (sem : (ev |= s => ev')%extgmpssem f) : P ev s ev' :=
-        match s in (_gmp_stmt_sem _ _ g0 e0) return (P g0 e0) with
-        | S_init _ _ x l u x0 x1 => P1 x l u x0 x1
-        | S_clear _ _ x a u x0 => P2 x a u x0
-        | S_set_i _ _ x y z a x0 x1 => P3 x y z a x0 x1
-        | S_set_z _ _ x y z a n x0 x1 x2 => P4 x y z a n x0 x1 x2
-        | S_get_int _ _ x y ly zy ir x0 x1 => P5 x y ly zy ir x0 x1
-        | S_set_s _ _ s x zx lx x0 x1 => P6 s x zx lx x0 x1
-        | S_cmp _ _ c x lx ly zx y zy b x0 x1 x2 x3 x4 =>
-            P7 c x lx ly zx y zy b x0 x1 x2 x3 x4
-        | S_op _ _ bop r lr x y lx ly zx zy x0 x1 x2 x3 x4 =>
-            P8 bop r lr x y lx ly zx zy x0 x1 x2 x3 x4
-        | S_Scope _ _ decls s ev_s ev_s' x x0 => P9 decls s ev_s ev_s' x x0
-        end *)
-
-
-
-    End Induction.
-
-    Definition gmp_stmt_sem := @generic_stmt_sem _gmp_statement _gmp_t _gmp_stmt_sem _gmp_stmt_vars.
+    Definition gmp_stmt_sem := @generic_stmt_sem _gmp_statement _gmp_t _gmp_stmt_sem _gmp_used_stmt_vars (fun _ => T_Ext Mpz).
 
     Definition gmp_pgrm_sem := 
-        @generic_pgrm_sem Empty_set _gmp_statement _gmp_t _gmp_stmt_sem _gmp_stmt_vars (fun _ => T_Ext Mpz)  build_rac_fenv.
+        @generic_pgrm_sem Empty_set _gmp_statement _gmp_t _gmp_stmt_sem _gmp_used_stmt_vars (fun _ => T_Ext Mpz)  build_rac_fenv.
 
 End GMPSemantics.
 
