Arithmetic/theories/Oracle.v
@@ -1,4 +1,6 @@
-From Coq Require Import ZArith.ZArith Strings.String Sets.Ensembles Sets.Finite_sets Orders Structures.OrdersEx.
+From Coq Require Import ZArith.ZArith Strings.String.
+From Coq.Structures Require Import Orders OrdersEx.
+From Coq.Sets Require Import Ensembles Finite_sets.
 From RAC Require Import Utils Environnement.
 From RAC.Languages Require Import Syntax Semantics.
 
@@ -6,23 +8,26 @@ From RAC.Languages Require Import Syntax Semantics.
 
 Module Type Oracle.
 
-    Definition 𝐼 : Type := Z ⨉ Z. (* interval *)
+    Definition interval : Type := Z ⨉ Z. (* interval *) (* using 𝐼 messes up vscoq *)
 
-    Definition Γᵢ : Type :=  StringMap.t 𝐼. (* typing env mapping logic binders to intervals *)
+    Definition Γᵢ : Type :=  StringMap.t interval. (* typing env mapping logic binders to intervals *)
 
     Parameter get_Γᵢ : fsl_pgrm -> Γᵢ. (* static analysis *)
 
-    Parameter oracle : ℨ ⨉ Γᵢ -> 𝐼. (* oracle *) (* using 𝓘 messes up vscoq *)
+    Parameter oracle : ℨ ⨉ Γᵢ -> interval. (* oracle *) (* using 𝓘 messes up vscoq *)
 
-    Parameter ϴ :  𝐼 -> 𝔗.
+    Parameter ty_from_interval :  interval -> 𝔗. (* using ϴ messes up vscoq *)
 
-    Parameter ϴ_int_or_mpz : forall i, ϴ i = C_Int \/  ϴ i = T_Ext Mpz.
+    Parameter ϴ_int_or_mpz : forall i, ty_from_interval i = C_Int \/  ty_from_interval i = T_Ext Mpz.
 
-    Definition get_ty : ℨ ⨉ Γᵢ -> 𝔗 := fun x => (ϴ  (oracle x)). (* using 𝒯 messes up vscoq *)
+    Definition get_ty : ℨ ⨉ Γᵢ -> 𝔗 := fun x => (ty_from_interval (oracle x)). (* using 𝒯 messes up vscoq *)
 
+
+    (* a program variable can't be an Mpz *)
+    Parameter get_ty_prog_var : forall x i, get_ty (T_Id x FSL_Int, i) = C_Int.
 
     Parameter ty_funcall_is_ty_body: 
-        forall (f : fsl_prog_fenv) fname xargs (targs:list ℨ) (iargs:list 𝐼) b, 
+        forall (f : fsl_prog_fenv) fname xargs (targs:list ℨ) (iargs:list interval) b, 
         StringMap.find fname f.(lfuns) = Some (xargs,b) ->
         forall te,
         List.Forall2 (fun e => eq (oracle (e,te))) targs iargs ->
@@ -31,7 +36,7 @@ Module Type Oracle.
 
     (* a term always fits in an mpz and only fits in a machine integer if it is in range *)
     Inductive fits (z:Z) : 𝔗 -> Prop := 
-    | InInt : Int.inRange z -> fits z C_Int
+    | InInt : MI.inRange z -> fits z C_Int
     | InMpz : fits z (T_Ext Mpz)
     .
 
@@ -45,7 +50,7 @@ Module Type Oracle.
         - `ty_funcall_is_ty_body` tells this is the same as typing the body with infered argument intervals
      *)
     Parameter convergence_of_lfuns_ty : 
-        forall fname (targs:list ℨ) (iargs:list 𝐼), 
+        forall fname (targs:list ℨ) (iargs:list interval), 
         forall (typing_envs : Ensemble Γᵢ)  (fe:Γᵢ), Ensembles.In Γᵢ typing_envs fe ->
         (exists ty te, get_ty (T_Call fname targs, te) = ty) -> 
         Finite_sets.Finite _ typing_envs
