Arithmetic/theories/Languages/MiniC/Facts.v
@@ -1,4 +1,4 @@
-From Coq Require Import FinFun.
+From Coq Require Import Logic.FinFun.
 From RAC Require Import Utils Environnement.
 From RAC.Languages Require Import Syntax MiniC.Semantics.
 
@@ -6,12 +6,13 @@ Import FunctionalEnv Domain Facts.
 
 
 Section GenericFacts.
-    Context {S T : Set} {ext_stmt_vars : S -> StringSet.t} {fe : @fenv S T}.
-    
+    Context {S T : Set} {fe : @fenv S T}.
+    Context {ext_used_stmt_vars : S -> StringSet.t} {ext_ty_val: 𝕍 -> @c_type T}.
+
     Variable (stmt_sem : forall f e, @generic_stmt_sem_sig S T f e).
 
     Notation generic_exp_sem := (fun e => @generic_exp_sem T e).
-    Notation generic_stmt_sem := (fun f e => @generic_stmt_sem _ _ stmt_sem ext_stmt_vars f e).
+    Notation generic_stmt_sem := (fun f e => @generic_stmt_sem _ _ stmt_sem ext_used_stmt_vars ext_ty_val f e).
 
 
     Fact untouched_var_same_eval_exp : 
@@ -41,8 +42,8 @@ Section GenericFacts.
     Qed.
 
     Fact untouched_var_same_eval_stmt : 
-        @_untouched_var_same_eval_stmt _ _ stmt_sem ext_stmt_vars fe ->
-        @_untouched_var_same_eval_stmt _ _ generic_stmt_sem ext_stmt_vars fe.
+        @_untouched_var_same_eval_stmt _ _ stmt_sem ext_used_stmt_vars fe ->
+        @_untouched_var_same_eval_stmt _ _ generic_stmt_sem ext_used_stmt_vars fe.
     Proof with auto with rac_hint.
         intros Hext ev ev' s x Hderiv [Hnotin Huservar]. induction Hderiv ; simpl in Hnotin; trivial.
         - simpl. autounfold with rac_hint. rewrite p_map_not_same... StringSet.D.fsetdec.
@@ -67,9 +68,9 @@ Section GenericFacts.
         4,5:
             apply IHe1 with (v:=VInt (z ⁱⁿᵗ z_ir)) (v':=VInt (z0 ⁱⁿᵗ z_ir0)) in H11 ; [|assumption] ; injection H11 as eqz ;
             apply IHe2 with (v:=VInt (z' ⁱⁿᵗ z'_ir)) (v':= VInt (z'0 ⁱⁿᵗ z'_ir0)) in H13; [|assumption] ;  injection H13 as eqz' ; subst ; now rewrite H14 in H7.
-        - f_equal. f_equal. now apply Int.mi_eq. 
+        - f_equal. f_equal. now apply MI.mi_eq. 
         - congruence.
-        - f_equal. f_equal. apply Int.mi_eq. simpl. f_equal.
+        - f_equal. f_equal. apply MI.mi_eq. simpl. f_equal.
             + apply IHe1 with (v:=VInt (z ⁱⁿᵗ z_ir)) (v':= VInt (z0 ⁱⁿᵗ z_ir0)) in H13; [|assumption]. now injection H13. 
             + apply IHe2 with (v:=VInt (z' ⁱⁿᵗ z'_ir)) (v':=VInt (z'0 ⁱⁿᵗ z'_ir0)) in H14; [|assumption]. now injection H14.
     Qed.
@@ -123,10 +124,14 @@ Section GenericFacts.
             subst. apply IHHderiv in Hsem. now subst.
         - inversion H0 ; subst... apply determinist_exp_eval in H... apply H in H2. injection H2 as H2. now subst.
         - inversion H1...
+
+        - inversion H0. subst. enough (ev_s0 = ev_s).
+            + subst. apply IHHderiv in H5. now subst.
+            + admit.
         - inversion H0. subst. unfold _determinist_stmt_eval in Hds. eapply Hds...
             + apply H.
             + apply H2. 
-    Qed.
+    Admitted.
 
 End GenericFacts.
 
@@ -134,9 +139,9 @@ End GenericFacts.
 Fact _determinist_c_exp_eval {T : Set} : @_determinist_exp_eval T Empty_exp_sem.
 Proof. easy. Qed.
 
-Fact _determinist_c_stmt_eval {S T : Set} {ext_stmt_vars} : 
-    @_determinist_stmt_eval S T Empty_exp_sem Empty_stmt_sem ext_stmt_vars.
+Fact _determinist_c_stmt_eval {S T : Set} {ext_used_stmt_vars} : 
+    @_determinist_stmt_eval S T Empty_exp_sem Empty_stmt_sem ext_used_stmt_vars.
 Proof. easy. Qed.
 
 
-(* Definition determinist_c_stmt_eval {S T } fe := @determinist_stmt_eval S T Empty_ext_stmt_vars fe Empty_stmt_sem  _determinist_c_stmt_eval. *)
+(* Definition determinist_c_stmt_eval {S T } fe := @determinist_stmt_eval S T Empty_ext_used_stmt_vars fe Empty_stmt_sem  _determinist_c_stmt_eval. *)
